Main.lean
@@ -256,7 +256,7 @@ def test_roundCircuitAgainstSmtlib (ein sin eout sout : Nat) : IO ExitCode := do
   let e2m4 : FPFormat := { e := ein, m := sin }
   let e2m2 : FPFormat := { e := eout, m := sout }
   let mut totalFailures := 0
-  for rm in [.RTP] do
+  for rm in allRoundingModes do
     IO.println "==="
     IO.println s!"🧪 ROUNDING MODE {repr rm}"
     let mut nsuccess := 0
@@ -275,7 +275,7 @@ def test_roundCircuitAgainstSmtlib (ein sin eout sout : Nat) : IO ExitCode := do
           IO.println s!"    - (Q: {repr roundSmt.unpack.toExtRat}); {repr roundSmt.unpack}"
       else
         nfailure := nfailure + 1
-        if true || nfailure < 1000 then
+        if nfailure < 10 then
          IO.println s!""
          IO.println s!"  ❌({repr rm} (Q: {repr pf.unpack.toExtRat}); {repr pf.unpack}"
          IO.println s!"    - SMT-LIB  (Q: {repr roundSmt.unpack.toExtRat}); {repr roundSmt.unpack}"
